fairness/examples/comp/lib.v
@@ -1,0 +1,79 @@
+From iris.proofmode Require Import tactics.
+From trillium.program_logic Require Export weakestpre.
+From trillium.fairness.heap_lang Require Export lang lifting tactics proofmode.
+From trillium.fairness.heap_lang Require Import notation.
+
+Close Scope Z_scope.
+
+Section LibraryDefs.
+
+  Definition lib_model_impl: FairModel.
+    refine ({|
+        fmstate := nat;
+        fmrole := unit;
+        fmtrans s1 oρ s2 := s1 = 1 /\ s2 = 0;
+        live_roles s := if (decide (s = 1)) then {[ tt ]} else ∅;
+        (* fuel_limit _ := 25%nat; (* exact value; should relax its usage *) *)
+             |}).
+    intros. set_solver. 
+  Defined. 
+
+  (* simply to differentiate between group- and individual role *)
+  Definition lib_grole := unit.
+  Definition ρlg: lib_grole := tt. 
+
+  Definition ρl: fmrole lib_model_impl := tt.
+
+  Definition lib_model: LiveModel lib_grole lib_model_impl LSI_True := 
+    {| lm_fl _ := 5; |}.  
+  
+  Definition lib_fun: val.
+  Admitted.
+
+  Lemma lib_model_impl_lr_strong: FM_strong_lr lib_model_impl.
+  Proof. 
+    red. intros. simpl.
+    destruct st; [| destruct st]; set_solver. 
+  Qed. 
+
+  (* TODO: this is needed to prove lib termination; should extract this part *)
+  From trillium.fairness Require Import fair_termination trace_helpers trace_lookup. 
+
+  (* straightforward proof which can be done more idiomatically 
+     by providing FairTerminatingModel of library *)
+  Lemma lib_fair_term:
+    ∀ mtr: mtrace lib_model_impl, mtrace_fairly_terminating mtr. 
+  Proof.
+    red. intros mtr VALID FAIR. 
+    destruct mtr; [by exists 1| ].
+    destruct mtr; [by exists 2| ].
+    pose proof (mtrace_valid_steps' VALID 0) as STEP0.
+    pose proof (mtrace_valid_steps' VALID 1) as STEP1.
+    rewrite trace_lookup_0_cons in STEP0. simpl in STEP0. 
+    specialize (STEP0 _ _ _ eq_refl) as [-> ->].
+    rewrite trace_lookup_cons trace_lookup_0_cons in STEP1.
+    specialize (STEP1 _ _ _ eq_refl). by inversion STEP1.
+  Qed. 
+  
+End LibraryDefs.
+
+Global Opaque lib_model_impl. 
+Global Opaque lib_grole ρlg. 
+
+Section LibrarySpec.
+  Context `{EM: ExecutionModel heap_lang M} `{@heapGS Σ _ EM}.
+  Context `{PMPP: @PartialModelPredicatesPre (locale heap_lang) _ _ Σ lib_model_impl}.
+  (* Context {ifG: fairnessGS lib_model Σ}. *)
+  
+  Notation "'PMP'" := (fun Einvs => (PartialModelPredicates Einvs (EM := EM) (iLM := lib_model) (PMPP := PMPP) (eGS := heap_fairnessGS))).
+
+  Lemma lib_spec tid Einvs:
+    PMP Einvs -∗
+    {{{ partial_model_is 1 (PartialModelPredicatesPre := PMPP) ∗ 
+        has_fuels tid {[ ρl:=2 ]} (PMPP := PMPP)  }}}
+      lib_fun #() @ tid
+    {{{ RET #(); partial_mapping_is {[ tid := ∅ ]} ∗ 
+                 partial_free_roles_are {[ tt ]} }}}.
+  Proof using. Admitted.
+
+End LibrarySpec.
